\documentclass{article}
\usepackage{graphicx} % Required for inserting images
\usepackage{amsfonts}
\renewcommand{\baselinestretch}{1.5}

\title{ctmc3}
\author{Haim Lavi, 038712105}
\date{August 2025}

\begin{document}

\maketitle

\section{}
$dX_t=2X_tdB_t$, $X_0=3$.

We divide both sides of the equation by $X_t\Rightarrow\frac{dX_t}{X_t}=2dB_t$.

We set $Y_y:=\ln{X_t}$, and calculate partial derivatives,

$\frac{\partial{Y_n}}{\partial{t}}=\frac{\partial\ln{X_t}}{\partial{t}}=0$.

$\frac{\partial{Y_t}}{\partial{X_t}}=\frac{\partial\ln{X_t}}{\partial{X_t}}=\frac{1}{X_t}$.

$\frac{\partial^2{Y_t}}{\partial{X_t}^2}=\frac{\partial^2\ln{X_t}}{\partial{X_t}^2}=-\frac{1}{X_t^2}$.

\noindent
By Ito, we get,
\[dY_t=d\ln{X_t}=\frac{1}{X_t}dX_t+\frac{1}{2}\cdot-\frac{1}{X_t^2}(dX_t)^2=\frac{dX_t}{X_t}-\frac{1}{2X_t^2}(2X_tdB_t)^2=\]\[=\frac{dX_t}{X_t}-\frac{4X_t^2(dB_t)^2}{2X_t^2}=\frac{dX_t}{X_t}-2(dB_t)^2.\]

We use the identity $(dB_t)^2=dt$, and the equation $\frac{dX_t}{X_t}=2dB_t$, and we get,

$dY_t=d\ln{X_t}=\frac{dX_t}{X_t}-2dt=2dB_t-2dt$.

We integrate both sides, and add the constant $Y_0=\ln{X_0}$,

\[Y_t=2B_t-2t+Y_0\Rightarrow{\ln{X_t}-\ln{X_0}=2B_t-2t}\Rightarrow\]\[\Rightarrow\ln\frac{X_t}{X_0}=2B_t-2t\Rightarrow\frac{X_t}{X_0}=e^{2B_t-2t}\Rightarrow{X_t=X_0e^{2Bt-2t}}=3e^{2B_t-2t}.\]
\section{}
$X_t=\cos(t+B_t)$.

We reconstruct the equation using Ito.

Denote $F(t,B_t)=\cos(t+B_t)$.

We calculate partial derivatives,

$\frac{\partial{F}}{\partial{t}}=-\sin(t+B_t)$.

$\frac{\partial{F}}{\partial{B_t}}=-\sin(t+B_t)$.

$\frac{\partial^2{F}}{\partial{B_t}^2}=-\cos(t+B_t)$.

Setting $F(t,B_t)=\cos(t,B_t)=X_t$, we get,
\noindent
\[dX_t=dF(t,B_t)=\frac{\partial{F}}{\partial{t}}dt+\frac{\partial{F}}{\partial{B_t}}dB_t+\frac{1}{2}\cdot\frac{\partial^2{F}}{\partial{B_t}^2}(dB_t)^2=\]\[=-\sin(t+B_t)dt-\sin(t+B_t)dB_t+\frac{1}{2}\cdot-\cos(t+B_t)(dB_t)^2=\]\[=[-\sin(t+B_t)-\frac{1}{2}\cos(t+B_t)]dt-\sin(t+B_t)dB_t.\]

But $\cos(t+B_t)=X_t\Rightarrow{-\sin(t+Bt)=-\sqrt{1-\cos^2(t+Bt)}}=-\sqrt{1-X_t^2}$.

Hence, $dX_t=[-\sqrt{1-X_t^2}-\frac{1}{2}X_t]dt-\sqrt{1-X_t^2}dB_t$.
\section{}
$dX_t=(\alpha-\mu{X_t})dt+\sigma{dW_t}$, $\alpha,\mu,\sigma>0$, $X_0=\frac{\alpha}{\mu}$.

We bring the equation to the form $dX_t=-\mu(X_t-\tilde\alpha)dt+\sigma{dW_t}$, 

where $\tilde\alpha=\frac{\alpha}{\mu}$.

Set $Y_t:=(X_t-\tilde\alpha)e^{\mu{t}}$.

We calculate partial derivatives,

$\frac{\partial{Y_t}}{\partial{t}}=\mu(X_t-\tilde\alpha)e^{\mu{t}}$.

$\frac{\partial{Y_t}}{\partial{X_t}}=dX_te^{\mu{t}}$.

$\frac{\partial^2{Y_t}}{\partial{X_t}^2}=\frac{\partial{e^{\mu{t}}}}{\partial{X_t}^2}dX_t=0$.

Then by Ito, we get,

$dY_t=\mu(X_t-\tilde\alpha)e^{-\mu{t}}dt+e^{-\mu{t}}dX_t$.

But $dX_t=-\mu(X_t-\tilde\alpha)dt+\sigma{dW_t}\Rightarrow$

\[\Rightarrow{dY_t=\mu(X_t-\tilde\alpha)e^{\mu{t}}dt+e^{\mu{t}}(-\mu(X_t-\tilde\alpha)dt+\sigma{dW_t})}=\]\[=\sigma{e^{\mu{t}}}dW_t\Rightarrow{Y_t=\int_0^t\sigma{e^{\mu{s}}}dW_s}+Y_0=\sigma\int_0^t{e^{\mu{s}}}dW_s+(X_0-\tilde\alpha)e^{\mu\cdot{0}}.\]

But \[X_0=\frac{\alpha}{\mu}=\tilde\alpha\Rightarrow{Y_t=\sigma\int_0^t{e^{\mu{s}}}dW_s}\Rightarrow.\]

But \[X_t=Y_t{e^{-\mu{t}}}+\tilde\alpha=e^{-\mu{t}}\sigma\int_0^t{e^{\mu{s}}dW_s}+\tilde\alpha.\]

We calculate the expectation,

\[\mathbb{E}[X_t]=\mathbb{E}[e^{-\mu{t}}\sigma\int_0^t{e^{\mu{s}}dW_s}+\tilde\alpha].\]

But expectation is linear, so we get,

\[\mathbb{E}[X_t]=\mathbb{E}[e^{-\mu{t}}\sigma\int_0^t{e^{\mu{s}}dW_s}]+\mathbb{E}[\tilde\alpha]=\sigma\mathbb{E}[\int_0^t{e^{\mu(s-t)}dW_s}]+\tilde\alpha.\]

But the expectation of a Brownian motion is zero, so we get,

$\mathbb{E}[X_t]=\tilde\alpha=\frac{\alpha}{\mu}$.

This means that if we start at the mean value, then the expectation remains the same, which means that this process has the behavior of a martingale.

\[Var(X_t)=\mathbb{E}[(X_t-\mathbb{E}[X_t])^2]=\mathbb{E}[(\sigma\int_0^t{e^{\mu(s-t)}}+\tilde\alpha-\tilde\alpha)^2]=\]\[=\mathbb{E}[(\sigma\int_0^t{e^{\mu(s-t)}})^2].\]

But by Ito isometry, we get,
\[Var(X_t)=\sigma^2\int_0^t{e^{2\mu(s-t)}}ds.\]

But this is a standard integral, with no stochastic element, so we get,

\[Var(X_t)=\frac{\sigma^2}{2\mu}[e^{2\mu(s-t)}]_0^t=\frac{\sigma^2}{2\mu}[e^{2\mu\cdot{t-t}}-e^{-2\mu{t}}]=\frac{\sigma}{2\mu}[1-e^{-2\mu{t}}].\]
\end{document}
